\section{Proof of lemma \getrefnumber{lemma:lipschitz_unicycle}}

Let $g(\vect{e}, \vect{u})$ be the differential equation describing the
error of the motion of the unicycle with respect to a fixed desired
configuration, and $\mat{Q} = Q_{\mu\nu}$ a $3 \times 3$ matrix. Then

\begin{align}
  \|g(\vect{e}_1, \vect{u}) - g(\vect{e}_2, \vect{u})\|_{Q} &=
  \Bigg\|
  \begin{bmatrix}
    v \cos\theta_1 - v \cos\theta_2 \\
    v \sin\theta_1 - v \sin\theta_2 \\
    \omega - \omega
  \end{bmatrix}
  \Bigg\|_Q \\[2.5ex]
  &=\sqrt{v^2
   \begin{bmatrix}
     \cos\theta_1 - \cos\theta_2 & \sin\theta_1 - \sin\theta_2 & 0
   \end{bmatrix}
   Q
   \begin{bmatrix}
     \cos\theta_1 - \cos\theta_2 \\
     \sin\theta_1 - \sin\theta_2 \\
     0
   \end{bmatrix}
  \\[2.5ex]}
  &= \sqrt{v^2 (\cos\theta_1 - \cos\theta_2)\Big( (Q_{11}+Q_{12})(\cos\theta_1 - \cos\theta_2) +
                    (Q_{21}+Q_{22})(\sin\theta_1 - \sin\theta_2)\Big)}
\end{align}

From the mean value theorem we derive the following
\begin{align}
  \cos\theta_1 - \cos\theta_2 = -\sin\gamma (\theta_1 - \theta_2) \leq |\theta_1 - \theta_2 \\[2.5ex]|
  \sin\theta_1 - \sin\theta_2 = \cos\gamma (\theta_1 - \theta_2) \leq |\theta_1 - \theta_2|
\end{align}
where $\theta_1 \leq \gamma \leq \theta_2$. Hence
\begin{align}
  \|g(\vect{e}_1, \vect{u}) - g(\vect{e}_2, \vect{u})\|_{Q} &\leq
    \sqrt{v^2 |\theta_1 - \theta_2|
      \Big( (Q_{11}+Q_{12}) |\theta_1 - \theta_2|+ (Q_{21}+Q_{22}) |\theta_1 - \theta_2|\Big) \\[2.5ex]}
      &= \sqrt{v^2 |\theta_1 - \theta_2|^2 (Q_{1,1}+Q_{1,2}+Q_{2,1}+Q_{2,2}) \\[2.5ex]}
      &= v \sqrt{Q_{1,1}+Q_{1,2}+Q_{2,1}+Q_{2,2}} \cdot |\theta_1 - \theta_2 \\[2.5ex]|
      &\leq v_{max} \sqrt{Q_{1,1}+Q_{1,2}+Q_{2,1}+Q_{2,2}} \cdot |\theta_1 - \theta_2|
\end{align}
